HOL: move del_annot_corres out and apply it for inductive eg

HOL/panScript.sml
@@ -9,7 +9,7 @@ open arithmeticTheory;
 open listTheory pairTheory;
 open itreeTauTheory;
 
-open panItreeSemTheory;
+open panItreeSemTheory panItreePropsTheory;
 open panSemTheory; (* eval_def, byte stuff *)
 open panLangTheory; (* size_of_shape_def *)
 open panPtreeConversionTheory; (* parse_funs_to_ast *)
@@ -18,7 +18,6 @@ open pred_setTheory set_relationTheory fixedPointTheory companionTheory;
 (* open set_sepTheory; *)
 
 (* can only load from here XXX bug? *)
-
 
 val _ = temp_set_fixity "≈" (Infixl 500);
 Overload "≈" = “itree_wbisim”;
@@ -92,7 +91,6 @@ Proof
   Cases_on ‘FLOOKUP s.code fname’ >> rw[byteTheory.bytes_in_word_def]
 QED
 
-Theorem itree_wbisim_refl[simp] = itree_wbisim_refl;
 Theorem apply_update_simp[simp] = cj 1 combinTheory.UPDATE_APPLY;
 (* may explode cases if k1 = k2 isn't decidable: luckily we cmp names = strings *)
 Theorem do_flookup_simp[simp] = finite_mapTheory.FLOOKUP_UPDATE;
@@ -122,222 +120,6 @@ Theorem mrec_sem_simps[simp] = panItreeSemTheory.mrec_sem_simps;
 val assign_tac = gvs[Once h_prog_def, h_prog_assign_def, eval_def];
 val strb_tac = rw[Once h_prog_def, h_prog_store_byte_def];
 
-(*
- * TODO put this metatheorem in props after miki converts the proofs
- *)
-
-Theorem mrec_sem_monad_law:
-  mrec_sem (ht >>= k)  =  (mrec_sem ht) >>= mrec_sem o k
-Proof
-  cheat
-QED
-
-Definition del_annot_def:
-  del_annot (Seq (Annot _ _) (p : 'a panLang$prog)) = del_annot p ∧
-  del_annot (Seq a b) = (Seq (del_annot a) (del_annot b)) ∧
-  del_annot (Dec vname e p) = (Dec vname e (del_annot p)) ∧
-  del_annot (DecCall m s e l p) = (DecCall m s e l (del_annot p)) ∧
-  del_annot (If gexp p1 p2) = (If gexp (del_annot p1) (del_annot p2)) ∧
-  del_annot (While gexp p) = (While gexp (del_annot p)) ∧
-  del_annot p = p
-End
-
-Theorem del_annot_seq_id:
-  (¬∃a b. p = Annot a b)
-  ⇒ del_annot (Seq p q) = Seq (del_annot p) (del_annot q)
-Proof
-  Cases_on ‘p’ >> rw[del_annot_def]
-QED
-
-Theorem prog_induct:
-  ∀P.
-    P Skip ∧ (∀p. P p ⇒ ∀e m. P (Dec m e p)) ∧
-    (∀m e. P (Assign m e)) ∧ (∀e e0. P (Store e e0)) ∧
-    (∀e e0. P (StoreByte e e0)) ∧ (∀p p0. P p ∧ P p0 ⇒ P (Seq p p0)) ∧
-    (∀p p0. P p ∧ P p0 ⇒ ∀e. P (If e p p0)) ∧
-    (∀p. P p ⇒ ∀e. P (While e p)) ∧ P Break ∧ P Continue ∧
-    (∀$o l e. P (Call $o e l)) ∧
-    (∀p. P p ⇒ ∀l e s m. P (DecCall m s e l p)) ∧
-    (∀m e e0 e1 e2. P (ExtCall m e e0 e1 e2)) ∧ (∀m e. P (Raise m e)) ∧
-    (∀e. P (Return e)) ∧ (∀ $o m e. P (ShMemLoad $o m e)) ∧
-    (∀$o e e0. P (ShMemStore $o e e0)) ∧ P Tick ∧
-    (∀m m0. P (Annot m m0))
-    ⇒ ∀p. P (p : 'a panLang$prog)
-Proof
-  strip_tac >>
-  qspecl_then [‘P’,‘K T’,‘K T’,‘K T’,‘K T’,‘K T’]
-              strip_assume_tac (cj 1 prog_induction) >>
-  rw[]
-QED
-
-(* this is surely true since no output is ever mapped above the error level
- * of its greatest 'element' in X, yet it is certainly not compatible
- * TODO maybe expand to: X ↦ ⋁ b^n X
- * note this is smaller than t ^, it does not approximate 'upwards'
- *)
-(* Theorem big_step_in_companion: *)
-(*   ∀X. *)
-(*     (λX. (λ(t,t'). *)
-(*             ∃h1 h2. *)
-(*               h1 ≈ h2 ∧ *)
-(*               t = h1 >>= k ∧ t' = h2 >>= k' ∧ *)
-(*               ∀a. (k a,k' a) ∈ X)) X *)
-(*     ⊆ set_companion wbisim_functional X *)
-(* Proof *)
-(*   strip_tac >> *)
-(*   irule set_compatible_enhance >> *)
-(*   qmatch_goalsub_abbrev_tac ‘f _ ⊆ _’ >> rw[] >> *)
-(*   qexists_tac ‘f’ >> *)
-(*   rw[set_compatible_def, monotone_def, Abbr ‘f’, SUBSET_DEF] >> *)
-(*   Cases_on ‘x’ >> fs[IN_DEF] >- (metis_tac[]) >> *)
-(*   fs[wbisim_functional_def] >> *)
-(*   (* h1 >>= k can branch to (Ret r) outside X? *) *)
-(*   rw[] *)
-(* QED *)
-
-Theorem whilebody_eq_corres:
-  (∀(s :(α, β) bstate). mrec_sem (h_prog (p,s)) ≈ mrec_sem (h_prog (p',s)))
-  ⇒ mrec_sem (h_prog (While e p,(s :(α, β) bstate)))
-  ≈ mrec_sem (h_prog (While e p',s))
-Proof
-  rw[h_prog_def, h_prog_while_def] >>
-  Cases_on ‘eval (reclock s) e’ >> rw[] >>
-  Cases_on ‘x’ >> rw[] >>
-  Cases_on ‘w’ >> rw[] >>
-  qmatch_goalsub_abbrev_tac ‘mrec_sem (_ >>= k) ≈ mrec_sem (_ >>= k')’ >>
-  rw[mrec_sem_monad_law] >>
-  ‘{mrec_sem (h_prog (p,s)) >>= mrec_sem ∘ k,
-   mrec_sem (h_prog (p',s)) >>= mrec_sem ∘ k'}
-            ⊆ rel_to_reln $≈’ suffices_by rw[SUBSET_DEF, rel_to_reln_def] >>
-  irule SUBSET_TRANS >>
-  qexists_tac ‘λ(a,b).
-                 (∃s. a = mrec_sem (h_prog (While e p,s)) ∧
-                      b = mrec_sem (h_prog (While e p',s))) ∨
-                 (∃t t'. t ≈ t' ∧
-                         a = t >>= mrec_sem ∘ k ∧
-                         b = t' >>= mrec_sem ∘ k')’ >>
-  rw[] >- (metis_tac[]) >>
-  rewrite_tac[GSYM wbisim_functional_gfp] >>
-  (* enhance avoids getting extra inductive cases on the after_tau! *)
-  irule set_param_coind_init >> conj_tac >- rw[] >>
-  irule set_param_coind >> conj_tac >- rw[] >>
-  qmatch_goalsub_abbrev_tac ‘set_companion _ target’ >>
-  rw[SUBSET_DEF, IN_DEF] >> Cases_on ‘x’ >> fs[] >-
-   (rw[h_prog_def, h_prog_while_def, SUBSET_DEF] >>
-    Cases_on ‘eval (reclock s') e’ >> rw[rel_to_reln_def] >-
-     (rw[wbisim_functional_def]) >>
-    reverse (Cases_on ‘x’) >> rw[] >- (rw[wbisim_functional_def]) >>
-    Cases_on ‘w’ >> rw[mrec_sem_monad_law, wbisim_functional_def] >>
-    disj2_tac >> rw[Abbr ‘target’] >>
-    irule singleton_subset >>
-    irule set_param_coind_done >>
-    rw[SUBSET_DEF] >> metis_tac[]) >>
-  rw[wbisim_functional_def] >>
-  pop_assum (strip_assume_tac o SRULE[Once itree_wbisim_cases]) >-
-   (disj2_tac >> fs[Abbr ‘target’] >>
-    irule singleton_subset >>
-    irule set_param_coind_done >> rw[] >>
-    metis_tac[]) >-
-   (disj1_tac >> disj2_tac >>
-    ‘strip_tau (t >>= mrec_sem ∘ k) (Vis e' (λx. k'' x >>= mrec_sem ∘ k))’
-      by metis_tac[itree_bind_vis_strip_tau] >>
-    ‘strip_tau (t' >>= mrec_sem ∘ k') (Vis e' (λx. k'³' x >>= mrec_sem ∘ k'))’
-      by metis_tac[itree_bind_vis_strip_tau] >>
-    qexistsl_tac[‘e'’,‘λx. k'' x >>= mrec_sem ∘ k’,‘λx. k'³' x >>= mrec_sem ∘ k'’]>>
-    rw[] >>
-    irule singleton_subset >>
-    irule set_param_coind_done >> rw[Abbr ‘target’] >>
-    metis_tac[]) >>
-
-  reverse (subgoal ‘(∃r'. strip_tau (Ret r >>= mrec_sem ∘ k) (Ret r') ∧
-                          strip_tau (Ret r >>= mrec_sem ∘ k') (Ret r')) ∨
-                    ∃t'' t'³'.
-                      (Ret r >>= mrec_sem ∘ k = Tau t'' ∧
-                       Ret r >>= mrec_sem ∘ k' = Tau t'³') ∧
-                      (t'',t'³') ∈ set_companion wbisim_functional target’) >-
-   (disj2_tac >>
-    qpat_assum ‘strip_tau t _’ mp_tac >>
-    Induct_on ‘strip_tau’ >> rw[] >-
-     (fs[] >>
-      irule singleton_subset >>
-      irule set_param_coind_upto >> rw[] >>
-      qexists_tac ‘after_taus_func’ >>
-      rw[in_after_taus_func] >>
-      irule after_taus_tauL >>
-      irule after_taus_rel >> rw[]) >>
-    qpat_assum ‘strip_tau t' _’ mp_tac >>
-    Induct_on ‘strip_tau’ >> rw[] >-
-     (fs[] >>
-      irule singleton_subset >>
-      irule set_param_coind_upto >> rw[] >>
-      qexists_tac ‘after_taus_func’ >>
-      rw[in_after_taus_func] >>
-      irule after_taus_tauR >>
-      irule after_taus_rel >> rw[]) >>
-    fs[]) >-
-   (metis_tac[itree_bind_resp_t_wbisim, itree_wbisim_strip_tau_Ret,
-              itree_wbisim_sym, itree_wbisim_strip_tau_sym, itree_wbisim_refl]) >>
-  rw[Abbr ‘k’, Abbr ‘k'’] >>
-  Cases_on ‘r’ >> rw[] >>
-  Cases_on ‘q’ >> rw[] >-
-   (disj2_tac >>
-    irule singleton_subset >>
-    irule set_param_coind_done >> rw[Abbr ‘target’] >>
-    metis_tac[]) >>
-  Cases_on ‘x’ >> rw[] >>
-  (disj2_tac >>
-   irule singleton_subset >>
-   irule set_param_coind_done >> rw[Abbr ‘target’] >>
-   metis_tac[])
-QED
-
-Theorem del_annot_corres:
-  mrec_sem (h_prog (del_annot ast,s)) ≈ mrec_sem (h_prog (ast,s))
-Proof
-  qid_spec_tac ‘s’ >>
-  qid_spec_tac ‘ast’ >>
-  recInduct prog_induct >>
-  rw[del_annot_def] >-
-   (rw[h_prog_def, h_prog_dec_def] >>
-    Cases_on ‘eval (reclock s) e’ >> rw[] >>
-    rw[mrec_sem_monad_law] >>
-    irule itree_bind_resp_wbisim >> fs[]) >-
-   (Cases_on ‘∃a b. p = Annot a b’ >> rw[] >-
-     (fs[h_prog_seq_def, h_prog_def, del_annot_def]) >>
-    fs[del_annot_seq_id] >>
-    rw[h_prog_def, h_prog_seq_def, del_annot_def] >>
-    rw[mrec_sem_monad_law] >>
-    irule itree_bind_resp_wbisim >> rw[] >>
-    Cases_on ‘r’ >> rw[]) >-
-   (rw[h_prog_def, h_prog_cond_def] >>
-    Cases_on ‘eval (reclock s) e’ >> rw[] >>
-    Cases_on ‘x’ >> rw[] >>
-    Cases_on ‘w’ >> rw[]) >-
-   (metis_tac[whilebody_eq_corres]) >-
-   (rw[h_prog_def, h_prog_deccall_def] >>
-    Cases_on ‘eval (reclock s') e’ >> rw[] >>
-    Cases_on ‘x’ >> rw[] >>
-    Cases_on ‘w’ >> rw[] >>
-    Cases_on ‘OPT_MMAP (eval (reclock s')) l’ >> rw[] >>
-    Cases_on ‘lookup_code s'.code m' x’ >> rw[] >>
-    Cases_on ‘x'’ >> rw[] >>
-    rw[mrec_sem_monad_law] >>
-    irule itree_bind_resp_wbisim >> rw[] >>
-    Cases_on ‘r'’ >> Cases_on ‘q'’ >-
-     (rw[h_handle_deccall_ret_def]) >>
-    Cases_on ‘x'’ >> rw[h_handle_deccall_ret_def] >>
-    rw[mrec_sem_monad_law] >>
-    irule itree_bind_resp_wbisim >>
-    rw[])
-QED
-
-(*
- * predicate for backwards proof:
- * if inv holds in all branches satisfying the postcondition, then it holds here
- *
- * problem: if post can be made to hold in all Ret branches, then it holds here
- *)
-
 Definition triple:
   triple inv (p,s) post =
   (∀k. (∀a. post a ⇒ inv (k a))
@@ -345,67 +127,15 @@ Definition triple:
        inv (mrec_sem (h_prog (p,s)) >>= k))
 End
 
-CoInductive silent:
-  silent (Ret r) ∧
-  (silent t ⇒ silent (Tau t))
+Definition resp_wbisim_def:
+  resp_wbisim P = (∀t t'. t ≈ t' ⇒ P t ⇒ P t')
 End
 
-Theorem silent_tau[simp]:
-  silent (Tau t) ⇔ silent t
+Theorem resp_wbisim_tau:
+  resp_wbisim P ⇒ (P (Tau t) ⇔ P t)
 Proof
-  rw[Once silent_cases]
-QED
-
-val silent = “silent :(32, β) stree -> bool”
-Theorem part1:
-  triple ^silent (panLang$While (Const 1w) Skip,s) (K F)
-Proof
-  rw[triple] >>
-  irule silent_coind >>
-  qexists_tac ‘λt. t = (mrec_sem (h_prog (While (Const 1w) Skip,s))) >>= k ∨
-                   t = Tau (mrec_sem (h_prog (While (Const 1w) Skip,s)) >>= k)’ >>
-  rw[Once h_prog_def] >>
-  disj2_tac >>
-  simp[SimpL “$=”, h_prog_while_def, eval_def] >>
-  ‘1 ≠ 0 MOD dimword (:32)’ by EVAL_TAC >>
-  rw[]
-QED
-
-Theorem part2:
-  triple ^silent (panLang$Return (Const 1w),s)
-  (λ(r,s). r = SOME (Return (ValWord (1w : word32))))
-Proof
-  rw[triple] >>
-  simp[h_prog_def, h_prog_return_def, eval_def, size_of_shape_def]
-QED
-
-Theorem satisfied:
-  ^silent (mrec_sem $ h_prog (panLang$Return (Const (1w : word32)),s))
-Proof
-  assume_tac part2 >>
-  fs[triple] >>
-  pop_assum $ qspec_then ‘Ret’ strip_assume_tac >> fs[] >>
-  pop_assum irule >> rw[] >>
-  rw[Once silent_cases]
-QED
-
-(* counterexample by Johannes
- * this cannot happen in an infinite case since we must prove the invariant
- * holds of (inf >>= k) = inf given pred (k r) for some arbitrary function k
- * which is only possible if the itree domain is very small *)
-
-CoInductive silent':
-  silent' (Ret (SOME (Return (ValWord 2w)))) ∧
-  (silent' t ⇒ silent' (Tau t))
-End
-
-Theorem satisfied:
-  triple silent' (panLang$Return (Const 1w),s)
-  (λ(r,s). r = SOME (Return (ValWord (1w : word32))))
-Proof
-  rw[triple] >>
-  simp[h_prog_def, h_prog_return_def, eval_def] >>
-  rw[size_of_shape_def]
+  rw[resp_wbisim_def] >>
+  metis_tac[itree_wbisim_tau_eq, itree_wbisim_sym]
 QED
 
 val P = “P :(32, β) stree -> bool”;
@@ -444,6 +174,78 @@ Proof
   Cases >> rw[]
 QED
 
+(*
+ * predicate for backwards proof:
+ * if inv holds in all branches satisfying the postcondition, then it holds here
+ *
+ * weird: if post can be made to hold in all Ret branches, then it holds here
+ *)
+
+CoInductive silent:
+  silent (Ret r) ∧
+  (silent t ⇒ silent (Tau t))
+End
+
+Theorem silent_resp:
+  resp_wbisim silent
+Proof
+  rw[resp_wbisim_def] >>
+  irule silent_coind >>
+  qexists_tac ‘λt'. ∃t. t ≈ t' ∧ silent t’ >>
+  rw[] >- (metis_tac[]) >>
+  Cases_on ‘a0’ >> rw[] >-
+   (metis_tac[itree_wbisim_trans, itree_wbisim_tau_eq]) >>
+  ntac 2 (last_x_assum kall_tac) >>
+  gvs[Once itree_wbisim_cases, Once silent_cases] >>
+  pop_assum mp_tac >> pop_last_assum mp_tac >>
+  Induct_on ‘strip_tau’ >> rw[] >>
+  rw[Once silent_cases]
+QED
+
+Theorem silent_tau[simp]:
+  silent (Tau t) ⇔ silent t
+Proof
+  metis_tac[silent_resp, resp_wbisim_tau]
+QED
+
+val silent = “silent :(32, β) stree -> bool”
+Theorem spin_silent:
+  triple ^silent (panLang$While (Const 1w) Skip,s) (K F)
+Proof
+  rw[triple] >>
+  irule silent_coind >>
+  qexists_tac ‘λt. t = (mrec_sem (h_prog (While (Const 1w) Skip,s))) >>= k ∨
+                   t = Tau (mrec_sem (h_prog (While (Const 1w) Skip,s)) >>= k)’ >>
+  rw[Once h_prog_def] >>
+  disj2_tac >>
+  simp[SimpL “$=”, h_prog_while_def, eval_def] >>
+  ‘1 ≠ 0 MOD dimword (:32)’ by EVAL_TAC >>
+  rw[]
+QED
+
+(* weird case found by Johannes: k now needs to 'fix' the return postcondition
+ * This also cannot happen in an infinite case since we must prove the invariant
+ * holds of (inf >>= k) = inf given pred (k r) for some arbitrary function k
+ * which is only possible if the itree domain is very small *)
+
+CoInductive silent':
+  silent' (Ret (SOME (Return (ValWord 2w)))) ∧
+  (silent' t ⇒ silent' (Tau t))
+End
+
+Theorem satisfied:
+  triple silent' (panLang$Return (Const 1w),s)
+  (λ(r,s). r = SOME (Return (ValWord (1w : word32))))
+Proof
+  rw[triple] >>
+  simp[h_prog_def, h_prog_return_def, eval_def] >>
+  rw[size_of_shape_def]
+QED
+
+(*
+ * example: inductive predicate
+ *)
+
 val while_ast = parse_pancake ‘
 fun tri(1 i) {
   var n = 0;
@@ -454,11 +256,11 @@ fun tri(1 i) {
   return n;
 }’;
 
-val while_noannot = rhs $ concl $ SRULE[] $ EVAL “del_annot (fun_ast ^while_ast)”;
+val while_annot = rhs $ concl $ SRULE[] $ EVAL “(fun_ast ^while_ast)”;
 
 Definition while_sem_def:
   while_sem (s:('a,'ffi) panItreeSem$bstate) =
-  mrec_sem (h_prog (^while_noannot,s))
+  mrec_sem (h_prog (^while_annot,s))
 End
 
 Definition tri_def:
@@ -471,7 +273,17 @@ Inductive correct:
   (correct i t ⇒ correct i (Tau t))
 End
 
-Theorem correct_wf[simp]:
+Theorem correct_resp:
+  resp_wbisim (correct i)
+Proof
+  simp[resp_wbisim_def] >>
+  Induct_on ‘correct’ >> simp[] >>
+  simp[Once itree_wbisim_cases] >>
+  Induct_on ‘strip_tau’ >> rw[] >>
+  rw[Once correct_cases]
+QED
+
+Theorem correct_tau[simp]:
   correct i (Tau t) ⇔ correct i t
 Proof
   rw[Once correct_cases]
@@ -551,9 +363,14 @@ Proof
   assume_tac while_seq_triple >> rw[]
 QED
 
+val while_noannot = rhs $ concl $ SRULE[] $ EVAL “del_annot (fun_ast ^while_ast)”;
 Theorem while_correct:
   correct i (while_sem (s with locals := s.locals |+ («i», ValWord (n2w i))))
 Proof
+  irule (SRULE[resp_wbisim_def] correct_resp) >>
+  rw[while_sem_def] >>
+  irule_at Any del_annot_corres >>
+  rw[del_annot_def] >>
   rw[while_sem_def] >>
   assume_tac while_triple >>
   fs[triple] >>
@@ -563,7 +380,7 @@ Proof
   Cases_on ‘a’ >> fs[]
 QED
 
-
+(* coinductive example *)
 
 
 
